```math
\begin{cases}
  mg\hat{e}_x+T\hat{\lambda}=m\vec{a},\\
  \hat{\lambda}=\frac{-x\hat{e}_x+y\hat{e}_y}{\sqrt{x^2+y^2}},\\
  \vec{a}=\ddot{x}\hat{e}_x+\ddot{y}\hat{e}_y\\
  L=\sqrt{x^2+y^2}
\end{cases}
```

```math
\left(mg-\frac{T_x}{L}\right)\hat{e}_x+\left(\frac{T_y}{L}\right)\hat{e}_y=m\left(\ddot{x}\hat{e}_x+\ddot{y}\hat{e}_y\right)
```

```math
\frac{d}{dt}\left(x^2+y^2\right)=\frac{d}{dt}L^2
```

```math
2x\dot{x} + 2y\ddot{y} = 0
```

```math
\frac{d^2}{dt^2}\left(x^2+y^2\right) = \frac{d^2}{dt2}L^2
```

```math
2\dot{x}^2+2x\ddot{x}+2\dot{y}^2+2y\ddot{y}=0
```

```math
x\ddot{x}+y\ddot{y}=-\dot{x}^2-\dot{y}^2
```

```math
\begin{cases}
  m\ddot{x}+\frac{x}{L}T=mg,\\
  m\ddot{y}+\frac{y}{L}T=0,\\
  x\ddot{x}+y\ddot{y}=-\left(\dot{x}^2+\dot{y}^2\right)
\end{cases}
```

```math
\begin{bmatrix} m & 0 & \frac{x}{L} \\ 0 & m & \frac{y}{L} \\ x & y & 0 \end{bmatrix} \begin{bmatrix} \ddot{x} \\ \ddot{y} \\ T \end{bmatrix} = \begin{bmatrix} mg \\ 0 \\ -\left(\dot{x}^2+\dot{y}^2\right) \end{bmatrix}
```
